Enrich namespace parameters in ilist example

nola/examples/ilist.v
@@ -2,7 +2,7 @@
 
 From nola.examples Require Export con.
 From nola.rust_lang Require Export notation proofmode.
-Import ProeqvNotation FunPRNotation WpwNotation CsemNotation.
+Import ProeqvNotation FunPRNotation ModwNotation WpwNotation CsemNotation.
 
 Section ilist.
   Context `{!Csem CON JUDG Σ, !Jsem JUDG (iProp Σ), !lrustGS_gen hlc Σ,
@@ -12,61 +12,63 @@ Section ilist.
   (** ** Linked list *)
 
   (** [cif_ilist]: Formula for a list *)
-  Definition ilist_gen N (Φx : loc -pr> cif CON Σ)
+  Definition ilist_gen N N' (Φx : loc -pr> cif CON Σ)
     (Ilist : loc -pr> cif CON Σ) l : iProp Σ :=
-    inv_tok N (Φx l) ∗ inv_tok N (∃ l', ▷ (l +ₗ 1) ↦ #l' ∗ Ilist l')%cif.
-  Definition cif_ilist_gen N (Φx : loc -pr> cif CON Σ) Ilist
+    inv_tok N (Φx l) ∗ inv_tok N' (∃ l', ▷ (l +ₗ 1) ↦ #l' ∗ Ilist l')%cif.
+  Definition cif_ilist_gen N N' (Φx : loc -pr> cif CON Σ) Ilist
     : loc -pr> cif CON Σ :=
-    λ l, as_cif (λ _, ilist_gen N Φx Ilist l).
-  #[export] Instance cif_ilist_gen_productive {k N} :
-    Proper ((≡[<k]≡) ==> (≡[<k]≡) ==> (≡[k]≡)) (cif_ilist_gen N).
+    λ l, as_cif (λ _, ilist_gen N N' Φx Ilist l).
+  #[export] Instance cif_ilist_gen_productive {k N N'} :
+    Proper ((≡[<k]≡) ==> (≡[<k]≡) ==> (≡[k]≡)) (cif_ilist_gen N N').
   Proof.
     unfold cif_ilist_gen=>/= ?? eq ?? eq' ?.
     f_equiv; apply cif_inv_tok_productive; (destruct k as [|k]; [done|]);
       [apply eq|]=>/=.
     f_equiv=> ?. by f_equiv.
   Qed.
-  #[export] Instance cif_ilist_gen_productive' {N Φx} :
-    Productive (cif_ilist_gen N Φx).
+  #[export] Instance cif_ilist_gen_productive' {N N' Φx} :
+    Productive (cif_ilist_gen N N' Φx).
   Proof. move=> ?. exact: cif_ilist_gen_productive. Qed.
-  Definition cif_ilist N (Φx : loc -pr> cif CON Σ) : loc -pr> cif CON Σ :=
-    profix (cif_ilist_gen N Φx).
+  Definition cif_ilist N N' (Φx : loc -pr> cif CON Σ) : loc -pr> cif CON Σ :=
+    profix (cif_ilist_gen N N' Φx).
   (** Unfold [cif_ilist] *)
-  Lemma cif_ilist_unfold {N Φx l} :
-    cif_ilist N Φx l ≡ cif_ilist_gen N Φx (cif_ilist N Φx) l.
-  Proof. by rewrite /cif_ilist (profix_unfold (f:=cif_ilist_gen _ _) l). Qed.
+  Lemma cif_ilist_unfold {N N' Φx l} :
+    cif_ilist N N' Φx l ≡ cif_ilist_gen N N' Φx (cif_ilist N N' Φx) l.
+  Proof. by rewrite /cif_ilist (profix_unfold (f:=cif_ilist_gen _ _ _) l). Qed.
   (** Semantics *)
-  Definition ilist N Φx := ilist_gen N Φx (cif_ilist N Φx).
+  Definition ilist N N' Φx := ilist_gen N N' Φx (cif_ilist N N' Φx).
   (** Unfold semantics over [cif_ilist] *)
-  Lemma sem_ilist {δ N Φx l} : cif_sem δ (cif_ilist N Φx l) ⊣⊢ ilist N Φx l.
+  Lemma sem_ilist {δ N N' Φx l} :
+    cif_sem δ (cif_ilist N N' Φx l) ⊣⊢ ilist N N' Φx l.
   Proof. by rewrite cif_ilist_unfold /= !sem_cif_in /=. Qed.
   (** [cif_ilist] is productive *)
-  #[export] Instance cif_ilist_productive {N} : Productive (cif_ilist N).
+  #[export] Instance cif_ilist_productive {N N'} : Productive (cif_ilist N N').
   Proof. move=> ????. apply profix_preserv=> ?. by f_equiv. Qed.
 
   (** [cif_ilist_gen] is non-expansive *)
-  #[export] Instance cif_ilist_gen_ne {N} : NonExpansive2 (cif_ilist_gen N).
+  #[export] Instance cif_ilist_gen_ne {N N'} :
+    NonExpansive2 (cif_ilist_gen N N').
   Proof.
     unfold cif_ilist_gen=>/= ??*?*?. (do 3 f_equiv=>//)=> ?. by f_equiv.
   Qed.
-  #[export] Instance cif_ilist_gen_proper {N} :
-    Proper ((≡) ==> (≡) ==> (≡)) (cif_ilist_gen N).
+  #[export] Instance cif_ilist_gen_proper {N N'} :
+    Proper ((≡) ==> (≡) ==> (≡)) (cif_ilist_gen N N').
   Proof. apply ne_proper_2, _. Qed.
   (** [cif_ilist] is non-expansive *)
-  #[export] Instance cif_ilist_ne {N} : NonExpansive (cif_ilist N).
+  #[export] Instance cif_ilist_ne {N N'} : NonExpansive (cif_ilist N N').
   Proof. move=> ????. apply profix_ne=> ???. by f_equiv. Qed.
-  #[export] Instance cif_ilist_proper {N} :
-    Proper ((≡) ==> (≡)) (cif_ilist N).
+  #[export] Instance cif_ilist_proper {N N'} :
+    Proper ((≡) ==> (≡)) (cif_ilist N N').
   Proof. apply ne_proper, _. Qed.
 
   (** Access the tail of a list *)
   Definition tail_ilist : val := λ: ["l"], !ˢᶜ("l" +ₗ #1).
-  Lemma twp_tail_list {N E Φx l} : ↑N ⊆ E →
-    [[{ ilist N Φx l }]][inv_wsat ⟦⟧ᶜ]
+  Lemma twp_tail_list {N N' E Φx l} : ↑N ⊆ E → ↑N' ⊆ E →
+    [[{ ilist N N' Φx l }]][inv_wsat ⟦⟧ᶜ]
       tail_ilist [ #l] @ E
-    [[{ l', RET #l'; ilist N Φx l' }]].
+    [[{ l', RET #l'; ilist N N' Φx l' }]].
   Proof.
-    iIntros (? Ψ) "/= [_ #itl] →Ψ". wp_rec. wp_op.
+    iIntros (?? Ψ) "/= [_ #itl] →Ψ". wp_rec. wp_op.
     iMod (inv_tok_acc with "itl") as "/=[(%l' & >↦l' & ltl) cl]"; [done|].
     rewrite sem_ilist. iDestruct "ltl" as "#ltl". wp_read.
     iMod ("cl" with "[$↦l']") as "_". { by rewrite sem_ilist. }
@@ -77,35 +79,36 @@ Section ilist.
   Definition iter_ilist : val := rec: "self" ["f"; "c"; "l"] :=
     if: !"c" ≤ #0 then #☠ else
       "f" ["l"];; "c" <- !"c" - #1;; "self" ["f"; "c"; tail_ilist ["l"]].
-  Lemma twp_iter_list {N E Φx c l} {f : val} {n : nat} : ↑N ⊆ E →
+  Lemma twp_iter_list {N N' E Φx c l} {f : val} {n : nat} : ↑N ⊆ E → ↑N' ⊆ E →
     (∀ l', [[{ inv_tok N (Φx l') }]][inv_wsat ⟦⟧ᶜ] f [ #l'] @ E
       [[{ RET #☠; True }]]) -∗
-    [[{ c ↦ #n ∗ ilist N Φx l }]][inv_wsat ⟦⟧ᶜ]
+    [[{ c ↦ #n ∗ ilist N N' Φx l }]][inv_wsat ⟦⟧ᶜ]
       iter_ilist [f; #c; #l] @ E
     [[{ RET #☠; c ↦ #0 }]].
   Proof.
-    iIntros "% #f /=" (Ψ) "!> [c↦ #l] →Ψ".
+    iIntros "%% #f /=" (Ψ) "!> [c↦ #l] →Ψ".
     iInduction n as [|m] "IH" forall (l) "l".
     { wp_rec. wp_read. wp_op. wp_if. by iApply "→Ψ". }
     wp_rec. wp_read. wp_op. wp_if. wp_apply "f".
     { iDestruct "l" as "[$ _]". }
     iIntros "_". wp_seq. wp_read. wp_op. wp_write.
     have -> : (S m - 1)%Z = m by lia.
-    wp_apply twp_tail_list; [done..|]. iIntros (l') "#ltl".
+    wp_apply twp_tail_list; [|done..|]=>//. iIntros (l') "#ltl".
     iApply ("IH" with "c↦ →Ψ ltl").
   Qed.
 
   (** Iterate over a list with two threads *)
-  Lemma twp_fork_iter_list {N E Φx c' c l} {f : val} {m n : nat} : ↑N ⊆ E →
+  Lemma twp_fork_iter_list {N N' E Φx c' c l} {f : val} {m n : nat} :
+    ↑N ⊆ E → ↑N' ⊆ E →
     (∀ l', [[{ inv_tok N (Φx l') }]][inv_wsat ⟦⟧ᶜ] f [ #l'] @ E
       [[{ RET #☠; True }]]) -∗
-    [[{ c' ↦ #m ∗ c ↦ #n ∗ ilist N Φx l }]][inv_wsat ⟦⟧ᶜ]
+    [[{ c' ↦ #m ∗ c ↦ #n ∗ ilist N N' Φx l }]][inv_wsat ⟦⟧ᶜ]
       Fork (iter_ilist [f; #c'; #l]);; iter_ilist [f; #c; #l] @ E
     [[{ RET #☠; c ↦ #0 }]].
   Proof.
-    iIntros "% #f" (Ψ) "!> (↦' & ↦ & #l) →Ψ". wp_apply (twp_fork with "[↦']").
+    iIntros "%% #f" (Ψ) "!> (↦' & ↦ & #l) →Ψ". wp_apply (twp_fork with "[↦']").
     { iApply (twp_mask_mono _ E); [done|].
-      wp_apply (twp_iter_list with "f [$↦' $l //]"); [done|]. by iIntros. }
+      wp_apply (twp_iter_list with "f [$↦' $l //]"); [done..|]. by iIntros. }
     iIntros. wp_seq. by wp_apply (twp_iter_list with "f [$↦ $l //]").
   Qed.
 
@@ -115,10 +118,10 @@ Section ilist.
     if: !"k" ≤ #0 then #☠ else
       Fork (let: "c" := Alloc #1 in "c" <- Ndnat;; iter_ilist ["f"; "c"; "l"]);;
       "k" <- !"k" - #1;; "self" ["f"; "k"; "l"].
-  Lemma twp_forks_iter_list {N E Φx k l} {f : val} {n : nat} :
+  Lemma twp_forks_iter_list {N N' E Φx k l} {f : val} {n : nat} :
     (∀ l', [[{ inv_tok N (Φx l') }]][inv_wsat ⟦⟧ᶜ] f [ #l']
       [[{ RET #☠; True }]]) -∗
-    [[{ k ↦ #n ∗ ilist N Φx l }]][inv_wsat ⟦⟧ᶜ]
+    [[{ k ↦ #n ∗ ilist N N' Φx l }]][inv_wsat ⟦⟧ᶜ]
       forks_iter_list [f; #k; #l] @ E
     [[{ RET #☠; k ↦ #0 }]].
   Proof.
@@ -131,10 +134,10 @@ Section ilist.
     iIntros. wp_seq. wp_read. wp_op. have -> : (S m - 1)%Z = m by lia. wp_write.
     iApply ("IH" with "↦ →Ψ l").
   Qed.
-  Lemma twp_nd_forks_iter_list {N E Φx l} {f : val} :
+  Lemma twp_nd_forks_iter_list {N N' E Φx l} {f : val} :
     (∀ l', [[{ inv_tok N (Φx l') }]][inv_wsat ⟦⟧ᶜ] f [ #l']
       [[{ RET #☠; True }]]) -∗
-    [[{ ilist N Φx l }]][inv_wsat ⟦⟧ᶜ]
+    [[{ ilist N N' Φx l }]][inv_wsat ⟦⟧ᶜ]
       let: "k" := Alloc #1 in "k" <- Ndnat;; forks_iter_list [f; "k"; #l] @ E
     [[{ RET #☠; True }]].
   Proof.
